commented out current eo adequacy proof; switching to completing eo_fin

fairness/lawyer/examples/eo/eo_adequacy.v
@@ -1,54 +1,164 @@
 From iris.algebra Require Import auth gmap gset excl excl_auth.
 From iris.proofmode Require Import tactics.
-From trillium.fairness Require Import locales_helpers comp_utils trace_lookup fairness.
+From trillium.fairness Require Import locales_helpers comp_utils fairness.
 From trillium.fairness.heap_lang Require Import simulation_adequacy notation.
-From trillium.fairness.lawyer Require Import counter_model sub_action_em.
-
+From trillium.fairness.lawyer Require Import counter_model sub_action_em action_model.
+From trillium.fairness.lawyer.obligations Require Import obligations_model obligations_am obligations_em obligations_resources obls_fairness_preservation obls_refill_em obls_refill_model.
+From trillium.fairness.lawyer.counter Require Import counter_em.
+(* TODO: avoid importing  the other definition*)
+From trillium.fairness Require Import trace_lookup.
 
 Definition eo_prog: val.
 Admitted. 
 
-Definition eo_ex_progress (l: loc) (extr : heap_lang_extrace) :=
+Definition eo_ex_dom (l: loc) (extr : heap_lang_extrace) :=
   ∀ (i: nat), ∃ n c, extr S!! n = Some c /\ heap (c.2) !! l = Some #i. 
 
 Definition eo_ex_mono (l: loc) (extr : heap_lang_extrace) :=
-  ∀ n, ∃ c c' oτ (i j: nat),
-    extr !! n = Some (c, Some (oτ, c')) /\
+  ∀ n c c' oτ (NTH: extr !! n = Some (c, Some (oτ, c'))),
+  exists (i j: nat),
     heap c.2 !! l = Some #i /\
     heap c'.2 !! l = Some #j /\
     i <= j
 .
 
+Definition eo_ex_progress l extr :=
+  (∀ tid, fair_ex tid extr) -> eo_ex_dom l extr /\ eo_ex_mono l extr.
+
 Section EOAdequacy.
 
+  Context {DegO LevelO: ofe}.
+  Context `{OfeDiscrete DegO} `{OfeDiscrete LevelO} `{@LeibnizEquiv (ofe_car LevelO) (ofe_equiv LevelO)}.
+  Context {LIM_STEPS: nat}.
+
+  Let Degree := ofe_car DegO.
+  Let Level := ofe_car LevelO.
+  
+  Context (OP: ObligationsParams Degree Level (locale heap_lang) LIM_STEPS).
+  Let ASEMo := ObligationsASEM OP.
+  Let ASEMc := @CounterASEM heap_lang.
+
+  (* TODO: move *)
+  Instance is_act_of_obls_dec: forall a, Decision (is_action_of (ObligationsRefillAM OP) a).
+  Proof. Admitted. 
+  Instance is_act_of_cnt_dec: forall a, Decision (is_action_of CounterAM a).
+  Proof. Admitted. 
+
+  Let ASEM := ProdASEM (ASEM1 := ASEMo) (ASEM2 := ASEMc).
+  Let EM := TopAM_EM ASEM (fun {Σ} {aGS: asem_GS Σ} τ => obls OP τ ∅ (H3 := aGS.1)).
+  Let PM := ProdAM (ObligationsRefillAM OP) CounterAM.
+  Let M := AM2M PM.
+  
   Definition eoΣ: gFunctors.
-  Admitted. 
+  Admitted.
 
-  Theorem eo_progress
-    (l: loc)
-    (extr : heap_lang_extrace)
-    (Hexfirst : trfirst extr = ([eo_prog #0], {| heap := {[l:=#0]}; used_proph_id := ∅ |})):
-    (* (∀ tid, fair_ex tid extr) -> terminating_trace extr. *)
-    extrace_fairly_terminating extr. 
+  Definition eo_st_rel (l: loc) (c: cfg heap_lang) (δ: mstate M) :=
+    om_live_tids OP id locale_enabled c δ.1 /\
+    heap c.2 !! l = Some #(δ.2).
+
+  Let eo_lbl_match (oτ: olocale heap_lang) (aρ: mlabel M): Prop :=
+        from_option (fun ρ => match ρ with
+                           | inl τ' => oτ = Some $ locale_of_orm_lbl OP τ'
+                           | inr _ => False
+                           end) False aρ.2.
+    
+  Definition eo_traces_match (l: loc): extrace heap_lang -> trace (mstate M) (mlabel M) -> Prop :=
+    traces_match
+      eo_lbl_match
+      (eo_st_rel l)
+      locale_step
+      (@mtrans M).
+
+  Lemma eo_matching_traces_dom l extr mtr 
+    (VALID: extrace_valid extr)
+    (MATCH: eo_traces_match l extr mtr)
+    (FAIR: ∀ tid, fair_ex tid extr):
+    eo_ex_dom l extr.
   Proof using.
-    assert (heapGpreS eoΣ EM) as HPreG.
-    { apply _. }
-
-    destruct (trfirst extr) as [tp_ σ1] eqn:EX0. simpl in *. subst tp_.                
-    
-    set (s1 := init_om_state (EO_OP LIM) (trfirst extr)). 
-    
-    unshelve epose proof (simple_om_simulation_adequacy_terminate (EO_OP LIM) eofinΣ NotStuck
-                  _ _ _ _
-                  _ _ EX0) as FAIR_TERM; eauto.
-    { exact tt. }
-    { simpl. subst s1. rewrite EX0. apply init_om_state_init. }
-    
-    apply FAIR_TERM.
-    red. intros ?. iStartProof. iIntros "[HEAP INIT] !>".
-    iSplitL.
-    - admit.
-    - subst s1. rewrite EX0. iApply om_sim_RAH. 
   Admitted. 
+
+  Lemma eo_matching_traces_mono l extr mtr 
+    (VALID: extrace_valid extr)
+    (MATCH: eo_traces_match l extr mtr):
+    eo_ex_mono l extr.
+  Proof using.
+    red. intros.
+    pose proof (traces_match_trace_lookup_general _ _ n MATCH) as REL.
+    rewrite NTH in REL.
+    destruct (mtr !! n) eqn:NTH'; [| done].
+    simpl in REL. destruct p as [δ [[ρ δ']|]]; [| tauto].
+    simpl in REL. rewrite /eo_st_rel in REL.
+    destruct δ as [? m], δ' as [? m']. 
+    simpl in REL. destruct REL as ([? LOC] & LBL & [? LOC']).
+    do 2 eexists. repeat split; eauto.
+
+    eapply trace_valid_steps' in NTH'.
+    2: { eapply traces_match_valid2; eauto. }
+
+    (* TODO: try to extract lemmas about this PM's steps *)
+    simpl in NTH'. inversion NTH'; subst; try lia.
+    - inversion STEP2.
+    - inversion STEP2. subst. inversion STEP. lia.
+    - inversion STEP2.
+    - inversion STEP2. subst. inversion STEP. lia. 
+  Qed.
+
+  Lemma eo_matching_traces_progress l extr mtr 
+    (VALID: extrace_valid extr)
+    (MATCH: eo_traces_match l extr mtr):
+    eo_ex_progress l extr.
+  Proof using.
+    red. intros. split; eauto using eo_matching_traces_dom, eo_matching_traces_mono.
+  Qed.
+
+  (* Theorem eo_simulation_adequacy Σ *)
+  (*       (* `{hPre: !heapGpreS Σ EM} (s: stuckness) *) *)
+  (*       (* (e1: expr) σ1 (s1: mstate OM) (* p *) *) *)
+  (*       (* (INIT: obls_is_init_st OP ([e1], σ1) s1) *) *)
+  (*       (* (extr : heap_lang_extrace) *) *)
+  (*       (* (Hexfirst : trfirst extr = ([e1], σ1))    : *) *)
+  (*       `{hPre: !heapGpreS Σ EM} (s: stuckness) *)
+  (*       (e1: expr) σ1 (s1: mstate M) p *)
+  (*       (INIT: em_is_init_st ([e1], σ1) s1 (ExecutionModel := EM)) *)
+  (*       (extr : heap_lang_extrace) *)
+  (*       (* (Hvex : extrace_valid extr) *) *)
+  (*       (Hexfirst : trfirst extr = ([e1], σ1))    : *)
+  (*   (* rel_finitary (sim_rel LM) → *) *)
+  (*   wp_premise Σ s e1 σ1 s1 eofin_sim_rel (p: @em_init_param _ _ EM) ->  *)
+  (*   eo_ex_property l extr.  *)
+  (* Proof. *)
+  (*   rewrite /extrace_fairly_terminating. *)
+  (*   intros (* Hterm Hfb *) Hwp (* VALID *) VALID FAIR. *)
+
+  (*   destruct (om_simulation_adequacy_model_trace *)
+  (*               Σ _ e1 _ s1 _ INIT _ VALID Hexfirst Hwp) as (omtr&MATCH&OM0). *)
+
+  (*   eapply eo_matching_traces_progress; eauto.  *)
+  (* Qed. *)
+
+  (* Theorem eo_progress *)
+  (*   (l: loc) *)
+  (*   (extr : heap_lang_extrace) *)
+  (*   (Hexfirst : trfirst extr = ([eo_prog #0], {| heap := {[l:=#0]}; used_proph_id := ∅ |})): *)
+  (*   (* (∀ tid, fair_ex tid extr) -> terminating_trace extr. *) *)
+  (*   eo_ex_progress l extr.  *)
+  (* Proof using. *)
+  (*   assert (heapGpreS eoΣ EM) as HPreG. *)
+  (*   { admit. } *)
+    
+  (*   set (s1 := init_om_state (EO_OP LIM) (trfirst extr)).  *)
+    
+  (*   unshelve epose proof (simple_om_simulation_adequacy_terminate (EO_OP LIM) eofinΣ NotStuck *)
+  (*                 _ _ _ _ *)
+  (*                 _ _ EX0) as FAIR_TERM; eauto. *)
+  (*   { exact tt. } *)
+  (*   { simpl. subst s1. rewrite EX0. apply init_om_state_init. } *)
+    
+  (*   apply FAIR_TERM. *)
+  (*   red. intros ?. iStartProof. iIntros "[HEAP INIT] !>". *)
+  (*   iSplitL. *)
+  (*   - admit. *)
+  (*   - subst s1. rewrite EX0. iApply om_sim_RAH.  *)
+  (* Admitted.  *)
 
 End EOAdequacy.
